added simulations

models/oalts/Alts.v
@@ -1,38 +1,139 @@
 Require Import interfaces.Category.
 Require Import oalts.AsyncEvents.
 Require Import oalts.Sig.
-Require Import oalts.PTree.
+Require Import oalts.Tree.
+From Paco Require Import paco.
 
 Module ALTS. (* <: Category. *)
   Import AsyncEvents.  
-  Import Sig.
-  Import PTree.
+  Import Tree.
 
-  Record ALTS {A : sig} := {
+  Record alts {A : Type} := {
     states : Type;
-    trans : states -> [A^- + A^+] -> states -> Prop;
+    trans : states -> [A] -> states -> Prop;
   }.
-  Arguments ALTS : clear implicits.
+  Arguments alts : clear implicits.
 
   Section Beh.
-    Context {A : sig}.
-    Variable σ : ALTS A.
+    Context {A : Type}.
+    Variable σ : alts A.
 
     Inductive tau_star : states σ -> states σ -> Prop :=
     | tau_refl : forall s, tau_star s s
     | tau_step : forall s1 s2 s3, 
         trans σ s1 τ s2 -> tau_star s2 s3 -> tau_star s1 s3.
 
+    Lemma tau_star_trans : forall (s1 s2 s3 : states σ),
+      tau_star s1 s2 -> tau_star s2 s3 -> tau_star s1 s3.
+    Proof.
+      intros s1 s2 s3 H1 H2.
+      induction H1; auto.
+      econstructor; eauto.
+    Qed.
+
     (* τ* followed by visible step *)
-    Definition weak_trans (s : states σ) (ev : A^- + A^+) (s' : states σ) : Prop :=
+    Definition weak_trans (s : states σ) (ev : A) (s' : states σ) : Prop :=
       exists s'', tau_star s s'' /\ trans σ s'' (vis ev) s'.
 
-    CoFixpoint beh (s : states σ) : ptree A :=
+    CoFixpoint beh (s : states σ) : tree A :=
       go (
         StepF 
-          (X := { ev : A^- + A^+  &  { s' : states σ | weak_trans s ev s' }})
+          (X := { ev : A  &  { s' : states σ | weak_trans s ev s' }})
           (fun x => projT1 x)
           (fun x => beh (proj1_sig (projT2 x)))
       ).
   End Beh.
+
+  Section Sim.
+    Context {A B : Type} (f : m A B).
+    Variable σ : alts A.
+    Variable ρ : alts B.
+
+    (* Convention: σ states are s1, s2, etc. and ρ states are s1', s2', etc. *)
+
+    (* R comes before s1, s1' for paco compatibility *)
+    Definition alts_simF (R : states σ -> states ρ -> Prop)
+      (s1 : states σ) (s1' : states ρ) : Prop :=
+      (forall ev s2, trans σ s1 (vis ev) s2 ->
+        match f ev with
+        | 'ev' => exists s2', weak_trans ρ s1' ev' s2' /\ R s2 s2'
+        | τ => R s2 s1'
+        end) /\
+      (forall s2, trans σ s1 τ s2 -> R s2 s1').
+
+    Lemma alts_simF_mon : monotone2 alts_simF.
+    Proof.
+      unfold monotone2, alts_simF. intros s1 s1' R R' [Hvis Htau] LE.
+      split.
+      - intros ev s2 Htrans. specialize (Hvis ev s2 Htrans).
+        destruct (f ev) as [ev' |].
+        + destruct Hvis as [s2' [Hweak HR]]. exists s2'. split; auto.
+        + apply LE. exact Hvis.
+      - intros s2 Htrans. apply LE. apply Htau. exact Htrans.
+    Qed.
+
+    #[local] Hint Resolve alts_simF_mon : paco.
+
+    Definition alts_sim : states σ -> states ρ -> Prop :=
+      paco2 alts_simF bot2.
+
+    Proposition alts_simF_sim : forall s1 s1',
+      alts_simF alts_sim s1 s1' -> alts_sim s1 s1'.
+    Proof.
+      intros s1 s1' [Hvis Htau]. pfold. split.
+      - intros ev s2 Htrans. specialize (Hvis ev s2 Htrans).
+        destruct (f ev) as [ev' |].
+        + destruct Hvis as [s2' [Hweak HR]]. exists s2'. split; auto.
+        + left. exact Hvis.
+      - intros s2 Htrans. left. apply Htau. exact Htrans.
+    Qed.
+
+    Proposition alts_sim_simF : forall s1 s1',
+      alts_sim s1 s1' -> alts_simF alts_sim s1 s1'.
+    Proof.
+      intros s1 s1' H. punfold H. destruct H as [Hvis Htau]. split.
+      - intros ev s2 Htrans. specialize (Hvis ev s2 Htrans).
+        destruct (f ev) as [ev' |].
+        + destruct Hvis as [s2' [Hweak HR]]. exists s2'. split; auto.
+          destruct HR; auto. contradiction.
+        + destruct Hvis; auto. contradiction.
+      - intros s2 Htrans. specialize (Htau s2 Htrans).
+        destruct Htau; auto. contradiction.
+    Qed.
+
+    Lemma alts_sim_tau_star : forall s1 s2 s1',
+      alts_sim s1 s1' -> tau_star σ s1 s2 -> alts_sim s2 s1'.
+    Proof.
+      intros s1 s2 s1' Hsim Hstar.
+      induction Hstar.
+      - exact Hsim.
+      - apply alts_sim_simF in Hsim as [Hvis Htau].
+        apply IHHstar.
+        apply Htau. exact H.
+    Qed.
+
+  Theorem alts_sim_beh : forall s1 s1',
+    alts_sim s1 s1' -> sim f (beh σ s1) (beh ρ s1').
+  Proof.
+    pcofix CIH.
+    intros s1 s1' Hsim.
+    pfold. simpl.
+    intros [ev [s2 Hweak]]. simpl.
+    destruct Hweak as [s3 [Hstar Htrans]].
+    pose proof (alts_sim_tau_star s1 s3 s1' Hsim Hstar) as Hsim'.
+    apply alts_sim_simF in Hsim' as [Hvis Htau].
+    specialize (Hvis ev s2 Htrans).
+    destruct (f ev) as [ev' |] eqn:Hf.
+    + (* Visible case *)
+      destruct Hvis as [s2' [Hweak2 Hsim'']].
+      exists (existT _ ev' (exist _ s2' Hweak2)).
+      simpl. split.
+      * reflexivity.
+      * right. apply CIH. exact Hsim''.
+    + (* Tau case *)
+      right. apply CIH. exact Hvis.
+  Qed.
+
+  End Sim.
+
 End ALTS.
